format-version: 1.2
data-version: releases/2024-04-04
ontology: geocore
property_value: http://purl.org/dc/elements/1.1/contributor "Fernando Cicconeto" xsd:string
property_value: http://purl.org/dc/elements/1.1/contributor "Joel Luis Carbonera" xsd:string
property_value: http://purl.org/dc/elements/1.1/contributor "Luan Fonseca Garcia" xsd:string
property_value: http://purl.org/dc/elements/1.1/contributor "Lucas Valadares Vieira" xsd:string
property_value: http://purl.org/dc/elements/1.1/contributor "Mara Abel" xsd:string
property_value: http://purl.org/dc/elements/1.1/contributor "Mara Abel" xsd:string
property_value: http://purl.org/dc/elements/1.1/contributor "Michel Perrin" xsd:string
property_value: http://purl.org/dc/elements/1.1/contributor "Renata dos Santos Alvarenga" xsd:string
property_value: owl:versionInfo "2024-04-04" xsd:string

[Term]
id: BFO:0000001
name: entity
property_value: definition "(Elucidation) An entity is anything that exists or has existed or will exist" xsd:string
property_value: example "Julius Caesar; the Second World War; your body mass index; Verdi's Requiem" xsd:string
property_value: http://purl.org/dc/elements/1.1/identifier "001-BFO" xsd:string

[Term]
id: BFO:0000002
name: continuant
is_a: BFO:0000001 ! entity
disjoint_from: BFO:0000003 ! occurrent
property_value: definition "(Elucidation) A continuant is an entity that persists, endures, or continues to exist through time while maintaining its identity" xsd:string
property_value: example "A human being; a tennis ball; a cave; a region of space; someone's temperature" xsd:string
property_value: http://purl.org/dc/elements/1.1/identifier "008-BFO" xsd:string

[Term]
id: BFO:0000003
name: occurrent
is_a: BFO:0000001 ! entity
property_value: definition "(Elucidation) An occurrent is an entity that unfolds itself in time or it is the start or end of such an entity or it is a temporal or spatiotemporal region" xsd:string
property_value: example "As for process, history, process boundary, spatiotemporal region, zero-dimensional temporal region, one-dimensional temporal region, temporal interval, temporal instant." xsd:string
property_value: http://purl.org/dc/elements/1.1/identifier "077-BFO" xsd:string

[Term]
id: BFO:0000004
name: independent continuant
is_a: BFO:0000002 ! continuant
disjoint_from: BFO:0000020 ! specifically dependent continuant
property_value: definition "b is an independent continuant =Def b is a continuant & there is no c such that b specifically depends on c or b generically depends on c" xsd:string
property_value: example "An atom; a molecule; an organism; a heart; a chair; the bottom right portion of a human torso; a leg; the interior of your mouth; a spatial region; an orchestra" xsd:string
property_value: http://purl.org/dc/elements/1.1/identifier "017-BFO" xsd:string

[Term]
id: BFO:0000008
name: temporal region
is_a: BFO:0000003 ! occurrent
disjoint_from: BFO:0000011 ! spatiotemporal region
property_value: definition "(Elucidation) A temporal region is an occurrent over which processes can unfold" xsd:string
property_value: example "As for zero-dimensional temporal region and one-dimensional temporal region" xsd:string
property_value: http://purl.org/dc/elements/1.1/identifier "100-BFO" xsd:string

[Term]
id: BFO:0000011
name: spatiotemporal region
is_a: BFO:0000003 ! occurrent
property_value: definition "(Elucidation) A spatiotemporal region is an occurrent that is an occurrent part of spacetime" xsd:string
property_value: example "The spatiotemporal region occupied by the development of a cancer tumour; the spatiotemporal region occupied by an orbiting satellite" xsd:string
property_value: http://purl.org/dc/elements/1.1/identifier "095-BFO" xsd:string
property_value: scopeNote "'Spacetime' here refers to the maximal instance of the universal spatiotemporal region." xsd:string

[Term]
id: BFO:0000015
name: process
is_a: BFO:0000003 ! occurrent
property_value: altLabel "event" xsd:string
property_value: definition "(Elucidation) p is a process means p is an occurrent that has some temporal proper part and for some time t, p has some material entity as participant" xsd:string
property_value: example "An act of selling; the life of an organism; a process of sleeping; a process of cell-division; a beating of the heart; a process of meiosis; the taxiing of an aircraft; the programming of a computer" xsd:string
property_value: http://purl.org/dc/elements/1.1/identifier "083-BFO" xsd:string

[Term]
id: BFO:0000019
name: quality
is_a: BFO:0000020 ! specifically dependent continuant
property_value: definition "(Elucidation) A quality is a specifically dependent continuant that, in contrast to roles and dispositions, does not require any further process in order to be realized" xsd:string
property_value: example "The colour of a tomato; the ambient temperature of this portion of air; the length of the circumference of your waist; the shape of your nose; the shape of your nostril; the mass of this piece of gold" xsd:string
property_value: http://purl.org/dc/elements/1.1/identifier "055-BFO" xsd:string

[Term]
id: BFO:0000020
name: specifically dependent continuant
is_a: BFO:0000002 ! continuant
property_value: definition "b is a specifically dependent continuant =Def b is a continuant & there is some independent continuant c which is not a spatial region & which is such that b specifically depends on c" xsd:string
property_value: example "(with multiple bearers) John's love for Mary; the ownership relation between John and this statue; the relation of authority between John and his subordinates" xsd:string
property_value: example "(with one bearer) The mass of this tomato; the pink colour of a medium rare piece of grilled filet mignon at its centre; the smell of this portion of mozzarella; the disposition of this fish to decay; the role of being a doctor; the function of this heart to pump blood; the shape of this hole" xsd:string
property_value: http://purl.org/dc/elements/1.1/identifier "050-BFO" xsd:string

[Term]
id: BFO:0000024
name: fiat object part
is_a: BFO:0000040 ! material entity
property_value: definition "(Elucidation) A fiat object part b is a material entity & such that if b exists then it is continuant part of some object c & demarcated from the remainder of c by one or more fiat surfaces" xsd:string
property_value: example "The upper and lower lobes of the left lung; the dorsal and ventral surfaces of the body; the Western hemisphere of the Earth; the FMA:regional parts of an intact human body" xsd:string
property_value: http://purl.org/dc/elements/1.1/identifier "027-BFO" xsd:string

[Term]
id: BFO:0000027
name: object aggregate
is_a: BFO:0000040 ! material entity
property_value: definition "(Elucidation) An object aggregate is a material entity consisting exactly of a plurality (≥1) of objects as member parts which together form a unit" xsd:string
property_value: example "The aggregate of the musicians in a symphony orchestra and their instruments; the aggregate of bearings in a constant velocity axle joint; the nitrogen atoms in the atmosphere; a collection of cells in a blood biobank" xsd:string
property_value: http://purl.org/dc/elements/1.1/identifier "025-BFO" xsd:string
property_value: scopeNote "'Exactly' means that there are no parts of the object aggregate other than its member parts." xsd:string
property_value: scopeNote "The unit can, at certain times, consist of exactly one object, for example, when a wolf litter loses all but one of its pups, but it must at some time have a plurality of member parts." xsd:string

[Term]
id: BFO:0000030
name: object
is_a: BFO:0000040 ! material entity
property_value: definition "(Elucidation) An object is a material entity which manifests causal unity & is of a type instances of which are maximal relative to the sort of causal unity manifested" xsd:string
property_value: example "An organism; a fish tank; a planet; a laptop; a valve; a block of marble; an ice cube" xsd:string
property_value: http://purl.org/dc/elements/1.1/identifier "024-BFO" xsd:string
property_value: scopeNote "A description of three primary sorts of causal unity is provided in Basic Formal Ontology 2.0. Specification and User Guide" xsd:string

[Term]
id: BFO:0000031
name: generically dependent continuant
is_a: BFO:0000002 ! continuant
property_value: altLabel "g-dependent continuant" xsd:string
property_value: definition "(Elucidation) A generically dependent continuant is an entity that exists in virtue of the fact that there is at least one of what may be multiple copies which is the content or the pattern that multiple copies would share" xsd:string
property_value: example "The pdf file on your laptop; the pdf file that is a copy thereof on my laptop; the sequence of this protein molecule; the sequence that is a copy thereof in that protein molecule; the content that is shared by a string of dots and dashes written on a page and the transmitted Morse code signal; the content of a sentence; an engineering blueprint" xsd:string
property_value: http://purl.org/dc/elements/1.1/identifier "074-BFO" xsd:string

[Term]
id: BFO:0000035
name: process boundary
is_a: BFO:0000003 ! occurrent
property_value: definition "p is a process boundary =Def p is a temporal part of a process & p has no proper temporal parts" xsd:string
property_value: example "The boundary between the 2nd and 3rd year of your life" xsd:string
property_value: http://purl.org/dc/elements/1.1/identifier "084-BFO" xsd:string

[Term]
id: BFO:0000038
name: one-dimensional temporal region
is_a: BFO:0000008 ! temporal region
property_value: definition "(Elucidation) A one-dimensional temporal region is a temporal region that is a whole that has a temporal interval and zero or more temporal intervals and temporal instants as parts" xsd:string
property_value: example "The temporal region during which a process occurs" xsd:string
property_value: http://purl.org/dc/elements/1.1/identifier "103-BFO" xsd:string

[Term]
id: BFO:0000040
name: material entity
is_a: BFO:0000004 ! independent continuant
disjoint_from: BFO:0000141 ! immaterial entity
property_value: definition "(Elucidation) A material entity is an independent continuant has some portion of matter as continuant part" xsd:string
property_value: example "A human being; the undetached arm of a human being; an aggregate of human beings" xsd:string
property_value: http://purl.org/dc/elements/1.1/identifier "019-BFO" xsd:string

[Term]
id: BFO:0000140
name: continuant fiat boundary
is_a: BFO:0000141 ! immaterial entity
property_value: definition "(Elucidation) A continuant fiat boundary b is an immaterial entity that is of zero, one or two dimensions & such that there is no time t when b has a spatial region as continuant part & whose location is determined in relation to some material entity" xsd:string
property_value: example "As for fiat point, fiat line, fiat surface" xsd:string
property_value: http://purl.org/dc/elements/1.1/identifier "029-BFO" xsd:string

[Term]
id: BFO:0000141
name: immaterial entity
is_a: BFO:0000004 ! independent continuant
property_value: definition "b is an immaterial entity =Def b is an independent continuant which is such that there is no time t when it has a material entity as continuant part" xsd:string
property_value: example "As for fiat point, fiat line, fiat surface, site" xsd:string
property_value: http://purl.org/dc/elements/1.1/identifier "028-BFO" xsd:string

[Term]
id: BFO:0000145
name: relational quality
is_a: BFO:0000019 ! quality
property_value: definition "b is a relational quality =Def b is a quality & there exists c and d such that c and d are not identical & b specifically depends on c & b specifically depends on d" xsd:string
property_value: example "A marriage bond; an instance of love; an obligation between one person and another" xsd:string
property_value: http://purl.org/dc/elements/1.1/identifier "057-BFO" xsd:string

[Term]
id: GEOCORE:0000000
name: geological object
name: objeto geológico
def: "An object that is 'generated by' some 'geological process' and has at least one part 'constituted by' some 'earth material' that is not an 'earth fluid'." []
is_a: BFO:0000030 ! object
relationship: UFRGS:GeoCoreOntology_generated_by UFRGS:GeoCoreOntology_geological_process {all_only="true"} ! processo geológico
relationship: UFRGS:GeoCoreOntology_has_age UFRGS:GeoCoreOntology_geological_age ! idade geológica
property_value: IAO:0000116 "A geological object is a naturally occurring entity because a geological process\ngenerates it, and some earth material constitutes it. Thus, we can differentiate geological objects from artificial objects, such as a well-core, because even though some earth material constitutes artificial objects, they are human-made rather than generated by some geological process. Furthermore, Geological Objects are specializations of BFO Objects, meaning they must necessarily have some unity criteria. The unity is what differentiates geological objects from Earth Materials." xsd:string

[Term]
id: UFRGS:GeoCoreOntology_earth_fluid
name: earth fluid
name: fluido da terra
def: "Earth fluid is an 'earth material' that is fluild." []
is_a: UFRGS:GeoCoreOntology_earth_material ! material geologico
disjoint_from: UFRGS:GeoCoreOntology_mineral ! quantidade de mineral
disjoint_from: UFRGS:GeoCoreOntology_mineral ! quantidade de mineral
disjoint_from: UFRGS:GeoCoreOntology_rock ! amount of rock
property_value: IAO:0000116 "Earth fluids can be water, oil, gas or a mixture of those fluids." xsd:string

[Term]
id: UFRGS:GeoCoreOntology_earth_material
name: earth material
name: material geologico
def: "It is a natural amount of matter 'generated by' some 'geological process'." []
is_a: BFO:0000040 ! material entity
relationship: UFRGS:GeoCoreOntology_generated_by UFRGS:GeoCoreOntology_geological_process {all_only="true"} ! processo geológico
property_value: IAO:0000112 "Examples are an amount of sandstone, an amount of petroleum, an amount of\nnatural gas." xsd:string
property_value: IAO:0000116 "Earth Materials are natural amounts of matter. Thus, they come into existence by nature, without any artificial aid. Since they are amounts, they don’t hold unity criteria, but they are ontologically rigid and provide an identity criteria. Earth Materials and BFO Objects are disjoint. They are either solid, fluid, or unconsolidated. We usually observe earth materials when constituting other objects, such as an amount of rock constituting a geological unity or an amount of sand constituting a dune." xsd:string

[Term]
id: UFRGS:GeoCoreOntology_geological_age
name: geological age
name: idade geológica
def: "It is a quality that 'inheres in' a 'geological object' or 'earth material' that corresponds to the 'geological time interval' in which the 'geological process' that it was 'generated by' occupied." []
is_a: BFO:0000019 ! quality

[Term]
id: UFRGS:GeoCoreOntology_geological_boundary
name: geological boundary
name: limite geológico
def: "It is a fiat surface that is 'located in' the external surface of a 'geological object'." []
is_a: BFO:0000140 ! continuant fiat boundary
property_value: IAO:0000116 "The 'geological boundary' of a 'geological object' coincides with the complete physical discontinuity that delimits it." xsd:string

[Term]
id: UFRGS:GeoCoreOntology_geological_contact
name: contato geológico
name: geological contact
def: "It is a 'relational quality' that 'inheres in' two distinct 'geological object' that are 'externally connected with'" []
comment: There was some problem with the axiom asserting that the contanct depends on two different objects.\n\nWe have to check it better.
is_a: BFO:0000145 ! relational quality
property_value: IAO:0000116 "A geological contact exists when two distinct geological objects are externally\nconnected with, i.e., their external boundaries are physically adjacent. Objects that are in contact do not have any kind of proper parthood relationship between them." xsd:string

[Term]
id: UFRGS:GeoCoreOntology_geological_process
name: geological process
name: processo geológico
def: "It is a physical, or chemical, or biological, naturally occurring process that occurs on the Earth’s surface or subsurface and occupies some 'geological time interval'" []
is_a: BFO:0000015 ! process
property_value: IAO:0000112 "Examples are the process of deposition, the process of folding, a tectonic process, a sedimentary process." xsd:string
property_value: IAO:0000116 "Geological processes are macro processes that generate, transform, deform, transport, or destroy geological objects and earth materials. These processes are not necessarily atomic and may have other geological processes as parts." xsd:string

[Term]
id: UFRGS:GeoCoreOntology_geological_structure
name: estrutura geológica
name: geological structure
def: "It is a 'generically dependent continuant' that is the pattern of a non-atomic 'geological object''s internal arrangement." []
is_a: BFO:0000031 ! generically dependent continuant
relationship: UFRGS:GeoCoreOntology_generically_depends_on GEOCORE:0000000 ! objeto geológico
property_value: IAO:0000116 "Geological structures are general material patterns repeated in many geological\nobjects. The pattern comprises the material configuration and the mutual relationships of the object’s different parts. Structures result from one or a series of geological processes that generated or transformed the geological object they generically depend on. Thus, there is some historical dependence relation between the structure and this geological process, but what concretizes the structure is some complex quality inhering in the object, not the process." xsd:string

[Term]
id: UFRGS:GeoCoreOntology_geological_time_interval
name: geological time interval
name: intervalo de tempo geológico
def: "It is a BFO temporal interval that corresponds to a time interval within the Geological Time Scale." []
is_a: BFO:0000038 ! one-dimensional temporal region

[Term]
id: UFRGS:GeoCoreOntology_mineral
name: amount of mineral
name: quantidade de mineral
def: "An amount of rock is an 'earth material' that is a naturally occuring, inorganic, solid, homogeneous chemical compound with a crystalline structure." []
is_a: UFRGS:GeoCoreOntology_earth_material ! material geologico
property_value: IAO:0000112 "The amount of quarts that constitutes some grain, the amount of feldspar that is part of an amount of rock." xsd:string
property_value: IAO:0000116 "Amounts of mineral lack a unity criteria as every other 'earth material'. We usually observe them when they are constitution objects such as crystals or grains." xsd:string

[Term]
id: UFRGS:GeoCoreOntology_rock
name: amount of rock
name: quantidade de rocha
def: "An amount of rock is a solid consolidated 'earth material' that is 'constituted by' an aggregate of particles made of mineral matter or material of biological origin." []
is_a: UFRGS:GeoCoreOntology_earth_material ! material geologico
property_value: IAO:0000112 "The amount of sandstone that constitutes a lithostratigraphic unit." xsd:string
property_value: IAO:0000116 "Geologists define rocks at a scale of observation where they consider them homogeneous, even though an aggregate of solid particles constitutes it. These particles are usually geological objects, such as grains or crystals, or the rest of dead animals or plants. \n\nAmounts of rock, like other earth materials, are independent rigid entities that do not hold any unity criteria. We can observe them in nature when they are constituting objects such as geological unities." xsd:string

[Term]
id: UFRGS:GeoCoreOntology_unconsolidated_earth_material
name: material geológico inconsolidado
name: unconsolidated earth material
def: "Unconsolidated earth material is an 'earth material' that is consituted by an aggregate of solid particles but is not consolidated into a 'rock' it self." []
is_a: UFRGS:GeoCoreOntology_earth_material ! material geologico

[Typedef]
id: UFRGS:GeoCoreOntology_age_of
name: age of
def: "The relation between a Geological Age and a Geological Object. Inverse of has age relation." []
is_a: RO:0000080
inverse_of: UFRGS:GeoCoreOntology_has_age ! has age

[Typedef]
id: UFRGS:GeoCoreOntology_carrier_of
name: carrier of
def: "The relation between an independent continuant that is not a spatial region and is the carrier of some g-dependent continuant" []
property_value: IAO:0000112 "Molecules of DNA are carriers of genetic information" xsd:string
property_value: IAO:0000112 "This copy of War and Peace is carrier of the novel written by Tolstoy" xsd:string
property_value: IAO:0000112 "This hard drive is carrier of these data items" xsd:string
property_value: IAO:0000116 "This relation was defined in the BFO 2020 text. We added it in the GeoCore Ontology because the RO ontology didn't add it yet." xsd:string
property_value: IAO:0000119 "BFO 2020" xsd:string
domain: BFO:0000004 ! independent continuant
range: BFO:0000031 ! generically dependent continuant
inverse_of: UFRGS:GeoCoreOntology_generically_depends_on ! generically depends on

[Typedef]
id: UFRGS:GeoCoreOntology_constituted_by
name: constituted by
def: "The relation between some material entity and the material that it is made of." []
property_value: IAO:0000116 "This is a material constitution relation intended to represent the relationship between material objects, such as geological objects and earth materials, or aggregates of them." xsd:string
property_value: IAO:0000119 "Evnine, S. J. (2011). Constitution and composition: Three approaches to their relation. ProtoSociology, 27, 212-235." xsd:string
is_asymmetric: true

[Typedef]
id: UFRGS:GeoCoreOntology_generated_by
name: generated by
def: "A relation between an 'earth material' or 'geological object', and a process, in which the continuant was generated by the process" []
property_value: IAO:0000116 "When a geological process creates a new geological object or earth material, we\nsay that it generated this new geological object or earth material. Thus, every instance of earth material and geological object have a unique generation relation with one instance of geological process." xsd:string
range: UFRGS:GeoCoreOntology_geological_process ! processo geológico
is_a: RO:0000056
is_asymmetric: true

[Typedef]
id: UFRGS:GeoCoreOntology_generated_in
name: generated in
def: "The Geological Time Interval in which the object was generated." []

[Typedef]
id: UFRGS:GeoCoreOntology_generically_depends_on
name: generically depends on
def: "a g-dependent continuant b g-depends on an independent continuant c at t means: there inheres in c an s-dependent continuant which concretizes b at t" []
property_value: IAO:0000112 "The pattern shared by chess boards g-depends on any chess board." xsd:string
property_value: IAO:0000112 "The score of a symphony g-depends on a copy of the score." xsd:string
property_value: IAO:0000116 "This relation was defined in the BFO 2020 text. We added it in the GeoCore Ontology because the RO ontology didn't add it yet." xsd:string
property_value: IAO:0000118 "g-depends on" xsd:string
property_value: IAO:0000119 "BFO 2020" xsd:string
domain: BFO:0000031 ! generically dependent continuant
range: BFO:0000004 ! independent continuant

[Typedef]
id: UFRGS:GeoCoreOntology_has_age
name: has age
def: "The relation between a Geological Object and its Geological Age." []
is_a: RO:0000086

[Typedef]
id: UFRGS:GeologicalSpatialRelationsOntology_above
name: above
def: "A spatial relation between two Independent Continuants (BFO), x and y, in which x has a location greater than the location of y in the vertical axis corresponding to the same frame of reference. It is the inverse relation of Below." []
domain: BFO:0000004 ! independent continuant
range: BFO:0000004 ! independent continuant
inverse_of: UFRGS:GeologicalSpatialRelationsOntology_below ! below

[Typedef]
id: UFRGS:GeologicalSpatialRelationsOntology_behind
name: behind
def: "A spatial relation between two Independent Continuants(BFO), x and y, in which y has a location that makes it nearer than x in the longitudinal axis corresponding to the same frame of reference. It is the inverse relation of In Front Of." []
domain: BFO:0000004 ! independent continuant
range: BFO:0000004 ! independent continuant

[Typedef]
id: UFRGS:GeologicalSpatialRelationsOntology_below
name: below
def: "A spatial relation between two Independent Continuants (BFO), x and y, in which x has a location lower than the location of y in the vertical axis corresponding to the same frame of reference. It is the inverse relation of Above." []
domain: BFO:0000004 ! independent continuant
range: BFO:0000004 ! independent continuant

